Lean4Lean/Verify/Level.lean
@@ -1,12 +1,13 @@
 import Lean4Lean.Theory.VLevel
+import Lean4Lean.Level
+import Lean4Lean.Verify.Axioms
+import Std.Tactic.BVDecide
 
-namespace Lean4Lean
-open Lean
-
-namespace VLevel
+namespace Lean.Level
+open Lean4Lean
 
 -- variable (ls : List Name) in
--- def toLevel : VLevel → Level
+-- def _root_.Lean4Lean.VLevel.toLevel : VLevel → Level
 --   | .zero => .zero
 --   | .succ l => .succ l.toLevel
 --   | .max l₁ l₂ => .max l₁.toLevel l₂.toLevel
@@ -17,3 +18,135 @@ namespace VLevel
 
 -- theorem toLevel_inj {ls : List Name} (d : ls.Nodup)
 --     {l₁ l₂ : VLevel} (eq : l₁.toLevel ls = l₂.toLevel ls) : l₁ = l₂ := sorry
+
+def realHasParam : Level → Bool
+  | .param .. => true
+  | .zero | .mvar .. => false
+  | .succ l => l.realHasParam
+  | .max l₁ l₂ | .imax l₁ l₂ => l₁.realHasParam || l₂.realHasParam
+
+def realHasMVar : Level → Bool
+  | .mvar .. => true
+  | .zero | .param .. => false
+  | .succ l => l.realHasMVar
+  | .max l₁ l₂ | .imax l₁ l₂ => l₁.realHasMVar || l₂.realHasMVar
+
+theorem Safe.succ : Safe (.succ u) → Safe u := by simp [Safe, realDepth]; omega
+theorem Safe.max : Safe (.max u v) → Safe u ∧ Safe v := by
+  simp [Safe, realDepth, Nat.max_eq_max, Nat.max_lt]; omega
+theorem Safe.imax : Safe (.imax u v) → Safe u ∧ Safe v := Safe.max
+
+theorem mkData_depth (H : d < 2 ^ 24) : (mkData h d hmv hp).depth.toNat = d := by
+  rw [mkData, if_neg (Nat.not_lt.2 (Nat.le_sub_one_of_lt H)), Data.depth]
+  have : d.toUInt64.toUInt32.toNat = d := by simp; omega
+  refine .trans ?_ this; congr 2
+  rw [← UInt64.toBitVec_inj]
+  have : d.toUInt64.toNat = d := by simp; omega
+  have : d.toUInt64.toBitVec ≤ 0xffffff#64 := (this ▸ Nat.le_sub_one_of_lt H :)
+  have : h.toUInt32.toUInt64.toBitVec ≤ 0xffffffff#64 := Nat.le_of_lt_succ h.toUInt32.1.1.2
+  have hb : ∀ (b : Bool), b.toUInt64.toBitVec ≤ 1#64 := by decide
+  have := hb hmv; have := hb hp
+  change (
+    h.toUInt32.toUInt64.toBitVec +
+    hmv.toUInt64.toBitVec <<< 32#64 +
+    hp.toUInt64.toBitVec <<< 33#64 +
+    d.toUInt64.toBitVec <<< 40#64) >>> 40#64 = d.toUInt64.toBitVec
+  bv_decide
+
+theorem mkData_hasParam (H : d < 2 ^ 24) : (mkData h d hmv hp).hasParam = hp := by
+  rw [mkData, if_neg (Nat.not_lt.2 (Nat.le_sub_one_of_lt H))]
+  simp [Data.hasParam, (· == ·), ← UInt64.toBitVec_inj]
+  have : h.toUInt32.toUInt64.toBitVec ≤ 0xffffffff#64 := Nat.le_of_lt_succ h.toUInt32.1.1.2
+  have hb : ∀ (b : Bool), b.toUInt64.toBitVec ≤ 1#64 := by decide
+  have := hb hmv; have := hb hp
+  let L := ((
+    h.toUInt32.toUInt64.toBitVec +
+    hmv.toUInt64.toBitVec <<< 32#64 +
+    hp.toUInt64.toBitVec <<< 33#64 +
+    d.toUInt64.toBitVec <<< 40#64) >>> 33#64) &&& 1#64
+  change decide (L = 1#64) = hp
+  rw [show L = hp.toUInt64.toBitVec by bv_decide]
+  cases hp <;> decide
+
+theorem mkData_hasMVar (H : d < 2 ^ 24) : (mkData h d hmv hp).hasMVar = hmv := by
+  rw [mkData, if_neg (Nat.not_lt.2 (Nat.le_sub_one_of_lt H))]
+  simp [Data.hasMVar, (· == ·), ← UInt64.toBitVec_inj]
+  have : h.toUInt32.toUInt64.toBitVec ≤ 0xffffffff#64 := Nat.le_of_lt_succ h.toUInt32.1.1.2
+  have hb : ∀ (b : Bool), b.toUInt64.toBitVec ≤ 1#64 := by decide
+  have := hb hmv; have := hb hp
+  let L := ((
+    h.toUInt32.toUInt64.toBitVec +
+    hmv.toUInt64.toBitVec <<< 32#64 +
+    hp.toUInt64.toBitVec <<< 33#64 +
+    d.toUInt64.toBitVec <<< 40#64) >>> 32#64) &&& 1#64
+  change decide (L = 1#64) = hmv
+  rw [show L = hmv.toUInt64.toBitVec by bv_decide]
+  cases hmv <;> decide
+
+theorem Safe.depth_eq {l : Level} (hl : l.Safe) : l.depth = l.realDepth := by
+  simp [Safe] at hl
+  have {n a} : n + 1 < a → n < a := by omega
+  induction l <;> (try specialize this hl) <;>
+    simp_all [depth, data, mkData_depth, realDepth, Nat.max_lt]
+
+theorem Safe.hasParam_eq {l : Level} (hl : l.Safe) : l.hasParam = l.realHasParam := by
+  have depth_eq := @Safe.depth_eq; simp [Safe, depth] at depth_eq
+  simp [Safe] at hl
+  have {n a} : n + 1 < a → n < a := by omega
+  induction l <;> (try specialize this hl) <;>
+    simp_all [hasParam, data, mkData_hasParam, realHasParam, realDepth, Nat.max_lt]
+
+theorem Safe.hasMVar_eq {l : Level} (hl : l.Safe) : l.hasMVar = l.realHasMVar := by
+  have depth_eq := @Safe.depth_eq; simp [Safe, depth] at depth_eq
+  simp [Safe] at hl
+  have {n a} : n + 1 < a → n < a := by omega
+  induction l <;> (try specialize this hl) <;>
+    simp_all [hasMVar, data, mkData_hasMVar, realHasMVar, realDepth, Nat.max_lt]
+
+theorem ofLevel_of_not_realHasParam (Us) {l : Level}
+    (hl : l.realHasParam = false) (hmv : l.realHasMVar = false) :
+    ∃ u', VLevel.ofLevel Us l = some u' := by
+  induction l <;> simp_all [realHasParam, realHasMVar, VLevel.ofLevel, exists_comm]
+
+def getUndefParam.F (ps : List Name) (l : Level) : StateT (Option Name) Id Bool := do
+  if !l.hasParam || (← get).isSome then
+    return false
+  if let .param n := l then
+    if n ∉ ps then
+      set (some n)
+  return true
+
+theorem getUndefParam_none {l : Level} (hl : l.Safe) (hmv : l.realHasMVar = false) :
+    l.getUndefParam Us = none → ∃ u', VLevel.ofLevel Us l = some u' := by
+  suffices ∀ s, ((l.forEach (getUndefParam.F Us)).run s).snd = none → s = none ∧ _ from
+    (this _ · |>.2)
+  have {l} (hl : l.Safe) (hmv : l.realHasMVar = false)
+      {g} (H : ∀ {s'}, (g.run s').snd = none → s' = none ∧
+       ((getUndefParam.F Us l).run none = (true, none) → ∃ u', VLevel.ofLevel Us l = some u')) (s) :
+      ((do if (!(← getUndefParam.F Us l)) = true then pure PUnit.unit else g).run s).snd = none →
+      s = none ∧ ∃ u', VLevel.ofLevel Us l = some u' := by
+    simp; split <;> rename_i h
+    · simp; revert h
+      simp [getUndefParam.F]; split <;> [simp; split <;> [split <;> simp; simp]]
+      rintro rfl; simp at *
+      exact ofLevel_of_not_realHasParam Us (hl.hasParam_eq.symm.trans ‹_›) hmv
+    · refine fun h' => let ⟨h1, h2⟩ := H h'; have := ?_; ⟨this, h2 ?_⟩
+      · revert h h1
+        simp [getUndefParam.F]; split <;> [simp; split <;> [split <;> simp; simp]]
+      · revert h h1; subst s
+        cases (getUndefParam.F Us l).run none; simp; rintro rfl rfl; rfl
+  have lt {n a} : n + 1 < a → n < a := by omega
+  induction l with (
+    refine this hl hmv fun h => ?_; clear this
+    simp [realHasMVar, VLevel.ofLevel, *] at *)
+  | succ _ ih =>
+    have ⟨h, _, h1⟩ := ih hl.succ hmv _ h
+    exact ⟨h, fun _ => ⟨_, _, h1, rfl⟩⟩
+  | max _ _ ih1 ih2 | imax _ _ ih1 ih2 =>
+    have ⟨h, _, h2⟩ := ih2 hl.max.2 hmv.2 _ h
+    have ⟨h, _, h1⟩ := ih1 hl.max.1 hmv.1 _ h
+    exact ⟨h, fun _ => ⟨_, _, h1, _, h2, rfl⟩⟩
+  | param =>
+    simp [getUndefParam.F, hl.hasParam_eq, Id, realHasParam, List.indexOf_lt_length_iff, *]
+    split <;> simp [*]
+  | _ => simp [*]
