Lean4Lean/Std/Basic.lean
@@ -96,6 +96,32 @@ theorem List.foldl_congr
     (H : ∀ a, ∀ x ∈ l, f a x = g a x) : foldl f a l = foldl g a l := by
   induction l generalizing a <;> simp_all
 
+theorem List.indexOf_eq_length_iff [BEq α] [LawfulBEq α]
+    {a : α} {l : List α} : indexOf a l = length l ↔ a ∉ l := by
+  induction l with
+  | nil => exact iff_of_true rfl (not_mem_nil _)
+  | cons b l ih =>
+    simp only [length, mem_cons, indexOf_cons, eq_comm]
+    rw [cond_eq_if]
+    split <;> rename_i h <;> simp at h
+    · exact iff_of_false (by rintro ⟨⟩) fun H => H <| Or.inl h.symm
+    · simp only [Ne.symm h, false_or]
+      rw [← ih]
+      exact Nat.succ_inj'
+
+theorem List.indexOf_le_length [BEq α] [LawfulBEq α]
+    {a : α} {l : List α} : indexOf a l ≤ length l := by
+  induction l with | nil => exact Nat.le_refl _ | cons b l ih => ?_
+  simp only [length, indexOf_cons, cond_eq_if, beq_iff_eq]
+  by_cases h : b == a
+  · rw [if_pos h]; exact Nat.zero_le _
+  · rw [if_neg h]; exact Nat.succ_le_succ ih
+
+theorem List.indexOf_lt_length_iff [BEq α] [LawfulBEq α]
+    {a} {l : List α} : indexOf a l < length l ↔ a ∈ l :=
+  ⟨fun h => Decidable.byContradiction fun al => Nat.ne_of_lt h <| indexOf_eq_length_iff.2 al,
+   fun al => (Nat.lt_of_le_of_ne indexOf_le_length) fun h => indexOf_eq_length_iff.1 h al⟩
+
 instance [BEq α] [LawfulBEq α] : PartialEquivBEq α where
   symm h := by simp at *; exact h.symm
   trans h1 h2 := by simp at *; exact h1.trans h2
